Translation/Term/Lemmas.lean
@@ -28,7 +28,7 @@ theorem Translation.GlobalEnv.lookup_ty_sound {G : Surface.GlobalEnv} : -- maybe
   G.translate = some G' ->
   (∀ (x : String) (T : Surface.Ty) (Δ : Core.KindEnv),
     (Surface.lookup_type G x = some T) ->
-    ∃ T' b, (Core.lookup_type G' x = some T' ∧ T.translate G' Δ = some T' ∧ G'&Δ ⊢ T' : .base b)) := by
+    ∃ T' b, (Core.lookup_type G' x = some T' ∧ T.translate = T' ∧ G'&Δ ⊢ T' : .base b)) := by
 intro wf h1 i K Δ h2
 sorry
 
@@ -70,20 +70,15 @@ case _ ih =>
 case _ f a ih =>
   rw[Option.bind_eq_some_iff] at h5;
   rcases h5 with ⟨f', h5, h6⟩
-  rw[Option.bind_eq_some_iff] at h6
-  rcases h6 with ⟨a', h7, h8⟩
-  cases h8
+  cases h6
   rw[Option.bind_eq_some_iff] at h1
   rcases h1 with ⟨sp', h1, h8⟩
   cases h8
   replace ih := @ih sp'.1 sp'.2 f' h1 h5
   rcases ih with ⟨sp'', ih⟩
   simp [Core.Term.spine]
-  exists (sp'' ++ [Core.SpineElem.type a']); rw[Option.bind_eq_some_iff]
+  exists (sp'' ++ [Core.SpineElem.type a.translate]); rw[Option.bind_eq_some_iff]
   exists (sp'.fst , sp'')
-
-def Surface.TyEnv.translate (G : Core.GlobalEnv) (Δ : Core.KindEnv) (Γ : Surface.TyEnv) : Option (Core.TyEnv) := Γ.mapM (·.translate G Δ )
-
 
 theorem Translation.KindEnv.lift_sound  {Δ : Surface.KindEnv} {Δ' : Core.KindEnv} {K : Surface.Kind} {K'}:
   Δ.translate = Δ' ->
@@ -95,80 +90,50 @@ rw[Surface.KindEnv.translate] at h1
 simp [h1, h2]
 
 theorem Translation.TyEnv.kindenv_lift_sound
-  {Δ : Surface.KindEnv} {Δ' : Core.KindEnv}
-  {Γ : Surface.TyEnv} {Γ' : Core.TyEnv}
-  {K : Surface.Kind} {K' : Core.Kind}:
-  Γ.translate G' Δ' = some Γ' ->
-  K.translate = K' ->
-  Surface.KindEnv.translate (K::Δ) = (K'::Δ') ->
-  Surface.TyEnv.translate G' (K'::Δ') (Γ.map (·[+1])) = some (Γ'.map (·[+1]))
+  {Γ : Surface.TyEnv} :
+  Surface.TyEnv.translate (Γ.map (·[+1])) = Γ.translate.map (·[+1])
    := by
-intro h1 h2 h3
-simp [Surface.TyEnv.translate, Surface.TyEnv.mapM] at*
-induction Γ using List.mapM'.induct generalizing Γ' G' Δ' K'
-case _ => simp at *; assumption
+induction Γ <;> simp at *
 case _ hd tl ih =>
-  simp at h1;
-  rw[Option.bind_eq_some_iff] at h1
-  rcases h1 with ⟨T', h1, h2⟩
-  rw[Option.bind_eq_some_iff] at h2
-  rcases h2 with ⟨Γ', h2', h3⟩
-  cases h3
-  rw[List.mapM_cons, bind, instMonadOption]; simp
-  rw[Option.bind_eq_some_iff]
-  exists T'[+1]
   apply And.intro
-  · apply Translation.Ty.Weaken h1
-  · rw[Option.bind_eq_some_iff];
-    exists Γ'.map (·[+1]);
-    apply And.intro;
-    · simp; apply ih h2' h2 h3
-    · simp
-
+  apply Translation.Ty.Weaken rfl
+  apply ih
 
 theorem Translation.TyEnv.lift_sound
-  {G : Surface.GlobalEnv} {G' : Core.GlobalEnv}
-  {Δ : Surface.KindEnv} {Δ' : Core.KindEnv}
+  {G : Surface.GlobalEnv}
+  {Δ : Surface.KindEnv}
   {Γ : Surface.TyEnv} {Γ' : Core.TyEnv}
   {A : Surface.Ty} {A' : Core.Ty} :
-  Γ.translate G' Δ' = some Γ' ->
+  Γ.translate = Γ' ->
   G&Δ ⊢s A : .base b ->
-  A.translate G' Δ' = some A' ->
-  Surface.TyEnv.translate G' Δ' (A :: Γ)= some (A'::Γ') := by
+  A.translate = A' ->
+  Surface.TyEnv.translate (A :: Γ) = (A'::Γ') := by
 intro h1 j h2
-simp [Surface.TyEnv.translate, Surface.TyEnv.mapM, List.mapM_cons, bind, instMonadOption, Option.bind_eq_some_iff];
+simp [Surface.TyEnv.translate, List.map_cons];
 constructor
 · assumption
 · apply h1
 
 
-theorem Translation.TyEnv.sound {G : Core.GlobalEnv} {Δ : Core.KindEnv} {Γ : Surface.TyEnv} {Γ' : Core.TyEnv} :
-  Γ.translate G Δ = some Γ' ->
+theorem Translation.TyEnv.sound {Γ : Surface.TyEnv} {Γ' : Core.TyEnv} :
+  Γ.translate = Γ' ->
   (∀ (i : Nat) (T : Surface.Ty),
-     (Γ[i]? = some T) -> ∃ T', ((Γ'[i]? = some T') ∧ T.translate G Δ = some T')) := by
+     (Γ[i]? = some T) -> (Γ'[i]? = some T.translate)) := by
 intro h1 i T h2;
-induction Γ using List.mapM'.induct generalizing G Δ Γ' i <;> simp [Surface.TyEnv] at h2
+induction Γ generalizing Γ' i <;> simp [Surface.TyEnv] at h2
 case _ => cases h2
 case _ hT Γ ih =>
-  simp [Surface.TyEnv.translate, Surface.TyEnv.mapM, List.mapM_cons] at *
-  rw[Option.bind_eq_some_iff] at h1
-  rcases h1 with ⟨T', h1, h2⟩
-  rw[Option.bind_eq_some_iff] at h2
-  rcases h2 with ⟨Γ', h3, h4⟩
-  cases h4
+  simp [Surface.TyEnv.translate] at *
   cases i <;> simp [Surface.TyEnv, Surface.inst_getElem?_TyEnv, Core.TyEnv, Core.inst_getElem?_TyEnv] at *
-  case zero => subst h2; assumption
-  case succ n =>
-    replace ih := @ih G Δ Γ' h3 n h2
-    rcases ih with ⟨T', h4, h5⟩
-    exists T'
+  case zero => subst h2; subst Γ'; simp;
+  case succ n => subst Γ'; simp; exists T;
 
 
 
 theorem Translation.ValidTyHeadVariable.sound {G : Surface.GlobalEnv} :
   ⊢s G ->
   G.translate = some G' ->
-  T.translate G' Δ' = some T' ->
+  T.translate = T' ->
   Surface.ValidTyHeadVariable T (Surface.is_data G) ->
   Core.ValidTyHeadVariable T' (Core.is_data G') := by
 intro wf h1 h2 h3
@@ -187,39 +152,36 @@ apply And.intro
 theorem Translation.StableTypeMatch.sound :
   -- ⊢s G ->
   -- G.translate = some G' ->
-  T.translate G' Δ' = some T' ->
-  R.translate G' Δ' = some R' ->
+  Δ.translate = Δ' ->
+  T.translate = T' ->
+  R.translate = R' ->
   Surface.StableTypeMatch Δ T R ->
   Core.StableTypeMatch Δ' T' R' := by
-intro h1 h2 h3
-induction h3 generalizing Δ' T' R' <;> try simp [Surface.Ty.translate] at *
+intro h1 h2 h3 h4
+induction h4 generalizing Δ' T' R' <;> try simp [Surface.Ty.translate] at *
 case refl h =>
-  rw[h1] at h2; cases h2
-  have lem := Translation.Ty.Spine h h1
+  rw[h3] at h2; cases h2
+  have lem := Translation.Ty.Spine h h3
   rcases lem with ⟨sp, lem⟩
   apply Core.StableTypeMatch.refl lem
 case arrow Δ B R A h ih =>
-  rw[Option.bind_eq_some_iff] at h1
-  rcases h1 with ⟨A', h1, h3⟩
-  rw[Option.bind_eq_some_iff] at h3
-  rcases h3 with ⟨B', h3, h4⟩
-  cases h4
+  cases h2
   apply Core.StableTypeMatch.arrow
-  apply ih h3 h2
+  subst h1; subst R'; apply ih
 case all K Δ B R a ih =>
-  rw[Option.bind_eq_some_iff] at h1
-  rcases h1 with ⟨A', h1, h3⟩
-  cases h3
+  subst h2
+  subst Δ'
   apply Core.StableTypeMatch.all
-  apply ih h1
-  apply Translation.Ty.Weaken h2
+  simp [Surface.KindEnv.translate] at ih
+  rw[Translation.Ty.Weaken h3] at ih
+  apply ih
 
 
 theorem Translation.PrefixTypeMatch.sound :
   Δ.translate = Δ' ->
-  A.translate G' Δ' = some A' ->
-  T.translate G' Δ' = some T' ->
-  R.translate G' Δ' = some R' ->
+  A.translate = some A' ->
+  T.translate = some T' ->
+  R.translate = some R' ->
   Surface.PrefixTypeMatch Δ A T R ->
   Core.PrefixTypeMatch Δ' A' T' R' := by
 intro h1 h3 h4 h5 h6
@@ -231,31 +193,17 @@ case refl B x Δ T j =>
   apply Core.PrefixTypeMatch.refl
   assumption
 case arrow Δ V B T A j1 ih =>
-  rw[Option.bind_eq_some_iff] at h3
-  rcases h3 with ⟨A', h3, h6⟩
-  rw[Option.bind_eq_some_iff] at h6
-  rcases h6 with ⟨V', h6, h7⟩
-  cases h7
-  rw[Option.bind_eq_some_iff] at h4
-  rcases h4 with ⟨A', h4, h8⟩
-  rw[Option.bind_eq_some_iff] at h8
-  rcases h8 with ⟨B', h8, h9⟩
-  cases h9; rw[h3] at h4; cases h4
+  subst A'; subst T'; subst R'
   apply Core.PrefixTypeMatch.arrow
-  apply ih h1 h6 h8 h5
+  apply ih h1 rfl rfl rfl
 case all K Δ B V T h ih =>
-  rw[Option.bind_eq_some_iff] at h3
-  rcases h3 with ⟨B', h3, h6⟩
-  cases h6
-  rw[Option.bind_eq_some_iff] at h4
-  rcases h4 with ⟨V', h4, h8⟩
-  cases h8
+  subst A'; subst T'; subst Δ'; subst R'
   apply Core.PrefixTypeMatch.all
-  apply ih _ h3 h4
-  apply Translation.Ty.Weaken h5
-  apply Translation.KindEnv.lift_sound h1 rfl
-
-
+  apply ih
+  rw[Surface.KindEnv.translate]; simp
+  rfl
+  rfl
+  apply Translation.Ty.Weaken rfl
 
 
 theorem Translation.ValidHeadVariable.sound
@@ -265,7 +213,7 @@ theorem Translation.ValidHeadVariable.sound
   ⊢s G ->
   G.translate = some G' ->
   Δ.translate = Δ' ->
-  Γ.translate G' Δ' = Γ' ->
+  Γ.translate = Γ' ->
   t.translate G' Δ' Γ' = some t' ->
   Surface.ValidHeadVariable t (Surface.is_ctor G) ->
   Core.ValidHeadVariable t' (Core.is_ctor G') := by
@@ -293,307 +241,296 @@ theorem Translation.Term.Sound (G : Surface.GlobalEnv) :
   G.translate = some G' ->
   ⊢ G' ->
   Δ.translate = Δ' ->
-  Γ.translate G' Δ' = some Γ' ->
+  Γ.translate = Γ' ->
 
-  ∃ T', (T.translate G' Δ' = some T' ∧
-    ∃ t', t.translate G' Δ' Γ' = some t' ∧
-    t'.Determined ∧
-    G'&Δ',Γ' ⊢ t' : T') := by
+
+  ∃ t', t.translate G' Δ' Γ' = some t' ∧
+        t'.Determined ∧
+        G'&Δ',Γ' ⊢ t' : T.translate := by
 intro wf j h1 wfc h2 h3
 induction j generalizing Δ' Γ' <;> simp at *
 case var Γ x T Δ b h jk =>
-  have lem := Translation.TyEnv.sound h3 x T h
-  rcases lem with ⟨T', h4, h5⟩
+  have lem := Translation.TyEnv.sound h3
+  replace lem := lem x T h
   replace jk := Translation.Ty.sound wf ⟨jk, h1 , h2⟩
   rcases jk with ⟨K', T', h6, h7, h8⟩
   have h6' := Translation.Kind.sound_base (b := b);
   rcases h6' with ⟨b', h6'⟩;
   rw[h6'] at h6; subst h6
-  rw[h7] at h5; cases h5
-  exists T'
-  constructor
-  · assumption
-  · constructor
-    · unfold Core.Term.Determined; apply Core.VariantMissing.var
-    · apply Core.Typing.var; repeat assumption
+  apply And.intro
+  · apply Core.Term.Determined.var
+  · subst h7; apply Core.Typing.var lem h8
 case global x T Δ b Γ h4 j =>
   have lem := Translation.GlobalEnv.lookup_ty_sound wf h1 x T Δ' h4
   rcases lem with ⟨T', h4, h5, h6, h7⟩
-  exists T'
-  constructor
-  · assumption
-  · constructor
-    unfold Core.Term.Determined; apply Core.VariantMissing.global
-    apply Core.Typing.global;
-    assumption
-    assumption
+  apply And.intro
+  · apply Core.Term.Determined.global
+  · subst h6; apply Core.Typing.global h5 h7
 case lam Δ A b1 Γ t B j1 j2 ih =>
   have lemA := Translation.Ty.sound wf ⟨j1, h1, h2⟩
   rcases lemA with ⟨aK', A', h4a, h5a, h6a⟩
   have lem := Translation.TyEnv.lift_sound h3 j1 h5a
-  replace ih := @ih _ (A' :: Γ') h2  lem
-  rcases ih with ⟨B', h8, t', h10, h11, h12⟩
+  rcases ih with ⟨t', h10, h11, h12⟩
   have lem := Core.Typing.well_typed_terms_have_base_kinds wfc h12
+  subst A'
   rcases lem with ⟨_, jB'⟩
-  exists (A' -:> B'); rw[Option.bind_eq_some_iff]
+  subst Δ'
+  exists (λ[A.translate] t')
+  rw[Option.bind_eq_some_iff];
   apply And.intro
-  · exists A'
-    apply And.intro
-    · assumption
-    · rw[Option.bind_eq_some_iff]; exists B'
-  · exists (λ[A']t')
-    rw[Option.bind_eq_some_iff];
-    apply And.intro
-    exists A'; apply And.intro; assumption; rw[Option.bind_eq_some_iff]; exists t'
-    have h6' := Translation.Kind.sound_base (b := b1)
-    rcases h6' with ⟨b1', h6'⟩
-    subst aK'; rw[h6'] at h6a
-    apply And.intro
+  · exists t'
+  · apply And.intro
     · apply Core.Term.Determined.lam; assumption
-    · apply Core.Typing.lam (b := b1')
+    · have h6' := Translation.Kind.sound_base b1
+      rcases h6' with ⟨b1', h6'⟩
+      subst aK'; rw[h6'] at h6a
+      apply Core.Typing.lam (b := b1')
       assumption
-      assumption
+      apply h12
+
+
+  -- · apply h10
+  --
 case lamt Δ K P t Γ j1 j2 ih =>
   have lem := Translation.Ty.sound wf ⟨j1, h1, h2⟩
   rcases lem with ⟨K', T', h4, h5, h6⟩
-  simp at h5; rw[Option.bind_eq_some_iff] at h5;
-  rcases h5 with ⟨P', h7, h8⟩
-  cases h8; simp at h4; subst K'
-  exists (∀[K.translate]P')
-  rw[Option.bind_eq_some_iff]
-  constructor
-  · simp; assumption
-  · have lemK := Translation.KindEnv.lift_sound (K := K) (K' := K.translate) h2 rfl
-    have lemT := Translation.TyEnv.kindenv_lift_sound (K := K) (K' := K.translate) (Δ := Δ) (Δ' := Δ') h3 rfl lemK
-    simp at lemT ih;
-    replace ih := @ih (K.translate :: Δ') (Γ'.map (·[+1])) lemK lemT
-    rcases ih with ⟨P', h8, t', h9, h10, h11⟩
-    rw[h7] at h8; cases h8
-    exists (Λ[K.translate]t');
-    apply And.intro
-    · rw[Option.bind_eq_some_iff]; exists t'
-    · apply And.intro
-      · apply Core.Term.Determined.lamt; assumption
-      · apply Core.Typing.lamt; assumption; assumption
-case app Δ A Γ f B a j1 j2 j3 ih1 ih2 =>
-  have lem := Translation.Ty.sound wf ⟨j1, h1, h2⟩
-  rcases lem with ⟨K', A', e1, e2, e3⟩
-  simp at e1; subst K'
-  replace ih1 := ih1 h2 h3
-  rcases ih1 with ⟨T', ih1⟩
-  rw[Option.bind_eq_some_iff] at ih1
-  rcases ih1 with ⟨h4, f', h5, h6, h7⟩
-  rcases h4 with ⟨A', h8, h9⟩
-  rw[Option.bind_eq_some_iff] at h9
-  rcases h9 with ⟨B', h9, h10⟩
-  cases h10
-
-  replace ih2 := ih2 h2 h3
-  rcases ih2 with ⟨A', h10, a', h11, h12, h13⟩
-
-  rw[h8] at h10; cases h10
-  rw[h8] at e2; cases e2
-  exists B'
+  rcases ih with ⟨t', ih1, ih2, ih3⟩
+  subst T'; subst Δ'; subst Γ';
+  simp at *
+  exists (Λ[K.translate]t');
   apply And.intro
-  · assumption
-  · exists (f' • a')
-    rw[Option.bind_eq_some_iff];
+  · rw[Option.bind_eq_some_iff]; exists t'; simp[Surface.KindEnv.translate] at ih1;
     apply And.intro
-    · exists f'
-      apply And.intro
-      · assumption
-      · rw[Option.bind_eq_some_iff]; exists a'
-    · apply And.intro
-      · apply Core.Term.Determined.app; assumption; assumption
-      · apply Core.Typing.app;
-        assumption
-        assumption
-        assumption
+    sorry
+    rfl
+  · sorry
+  -- · rw[Option.bind_eq_some_iff]
+  -- · apply And.intro
+  --     · apply Core.Term.Determined.lamt; assumption
+  --     · apply Core.Typing.lamt; assumption; assumption
+
+case app Δ A Γ f B a j1 j2 j3 ih1 ih2 =>
+  sorry
+  -- have lem := Translation.Ty.sound wf ⟨j1, h1, h2⟩
+  -- rcases lem with ⟨K', A', e1, e2, e3⟩
+  -- simp at e1; subst K'
+  -- replace ih1 := ih1 h2 h3
+  -- rcases ih1 with ⟨T', ih1⟩
+  -- rw[Option.bind_eq_some_iff] at ih1
+  -- rcases ih1 with ⟨h4, f', h5, h6, h7⟩
+  -- rcases h4 with ⟨A', h8, h9⟩
+  -- rw[Option.bind_eq_some_iff] at h9
+  -- rcases h9 with ⟨B', h9, h10⟩
+  -- cases h10
+
+  -- replace ih2 := ih2 h2 h3
+  -- rcases ih2 with ⟨A', h10, a', h11, h12, h13⟩
+
+  -- rw[h8] at h10; cases h10
+  -- rw[h8] at e2; cases e2
+  -- exists B'
+  -- apply And.intro
+  -- · assumption
+  -- · exists (f' • a')
+  --   rw[Option.bind_eq_some_iff];
+  --   apply And.intro
+  --   · exists f'
+  --     apply And.intro
+  --     · assumption
+  --     · rw[Option.bind_eq_some_iff]; exists a'
+  --   · apply And.intro
+  --     · apply Core.Term.Determined.app; assumption; assumption
+  --     · apply Core.Typing.app;
+  --       assumption
+  --       assumption
+  --       assumption
 
 
 case appt Δ Γ f K P a P' j1 j2 e ih =>
-  replace ih := ih h2 h3
-  rcases ih with ⟨T', h4, h5⟩
-  rw[Option.bind_eq_some_iff] at h4
-  rcases h4 with ⟨Pk', h4, h6⟩
-  cases h6
-  rcases h5 with ⟨f', h6, h7, h8⟩
+  sorry
+  -- replace ih := ih h2 h3
+  -- rcases ih with ⟨T', h4, h5⟩
+  -- rw[Option.bind_eq_some_iff] at h4
+  -- rcases h4 with ⟨Pk', h4, h6⟩
+  -- cases h6
+  -- rcases h5 with ⟨f', h6, h7, h8⟩
 
-  have lem := Translation.Ty.sound wf ⟨j2, h1, h2⟩
-  rcases lem with ⟨K', A', h9, h10, h11⟩
-  subst K'
-  exists Pk'[su A' :: +0:_]
-  apply And.intro
-  · have lem := Surface.Typing.well_typed_terms_have_base_kinds wf j1;
-    rcases lem with ⟨_, lem⟩
-    cases lem; case _ jp =>
-    have lem := Translation.KindEnv.lift_sound (K := K) (K' := K.translate) h2 rfl
-    replace lem := Translation.Ty.sound wf ⟨jp, h1, lem⟩
-    rcases lem with ⟨bk, Pk', e1, e2, e3⟩
-    simp at e1; subst e1
-    rw[h4] at e2; cases e2
-    have lem := Translation.Ty.beta (P' := Pk') (K' := K.translate) wf j2 jp h1 h2 rfl h10 h4
-    subst e
-    assumption
+  -- have lem := Translation.Ty.sound wf ⟨j2, h1, h2⟩
+  -- rcases lem with ⟨K', A', h9, h10, h11⟩
+  -- subst K'
+  -- exists Pk'[su A' :: +0:_]
+  -- apply And.intro
+  -- · have lem := Surface.Typing.well_typed_terms_have_base_kinds wf j1;
+  --   rcases lem with ⟨_, lem⟩
+  --   cases lem; case _ jp =>
+  --   have lem := Translation.KindEnv.lift_sound (K := K) (K' := K.translate) h2 rfl
+  --   replace lem := Translation.Ty.sound wf ⟨jp, h1, lem⟩
+  --   rcases lem with ⟨bk, Pk', e1, e2, e3⟩
+  --   simp at e1; subst e1
+  --   rw[h4] at e2; cases e2
+  --   have lem := Translation.Ty.beta (P' := Pk') (K' := K.translate) wf j2 jp h1 h2 rfl h10 h4
+  --   subst e
+  --   assumption
 
-  exists f' •[ A']
-  · rw[Option.bind_eq_some_iff]
-    apply And.intro
-    · exists f'; apply And.intro
-      · assumption
-      · rw[Option.bind_eq_some_iff]; exists A'
-    · apply And.intro
-      · apply Core.Term.Determined.appt; assumption
-      · apply Core.Typing.appt
-        assumption
-        assumption
-        rfl
+  -- exists f' •[ A']
+  -- · rw[Option.bind_eq_some_iff]
+  --   apply And.intro
+  --   · exists f'; apply And.intro
+  --     · assumption
+  --     · rw[Option.bind_eq_some_iff]; exists A'
+  --   · apply And.intro
+  --     · apply Core.Term.Determined.appt; assumption
+  --     · apply Core.Typing.appt
+  --       assumption
+  --       assumption
+  --       rfl
 
 case mtch n Δ Γ s R c T CTy PTy pats cs sj vhvR cj vhvps patsj stmPTys csj ptms ih1 ih2 ih3 ih4 =>
-  replace ih1 := ih1 h2 h3
-  rcases ih1 with ⟨R', ih1, s', ih1b, ih1c, ih1d⟩
-  replace ih2 := ih2 h2 h3
-  rcases ih2 with ⟨T', ih2, c', ih2b, ih2c, ih2d⟩
+  sorry
+  -- replace ih1 := ih1 h2 h3
+  -- rcases ih1 with ⟨R', ih1, s', ih1b, ih1c, ih1d⟩
+  -- replace ih2 := ih2 h2 h3
+  -- rcases ih2 with ⟨T', ih2, c', ih2b, ih2c, ih2d⟩
 
-  replace ih3 : ∃ (PTy' : Vect n Core.Ty),
-          (∀ (i : Fin n), Surface.Ty.translate G' Δ' (PTy i) = some (PTy' i)) ∧
-          ∃ (pats' : Vect n Core.Term),
-          (∀ i, Surface.Term.translate G' Δ' Γ' (pats i) = some (pats' i)) ∧
-          (∀ i, (pats' i).Determined) ∧
-          (∀ i, G'&Δ',Γ' ⊢ (pats' i) : (PTy' i)) := by
+  -- replace ih3 : ∃ (PTy' : Vect n Core.Ty),
+  --         (∀ (i : Fin n), Surface.Ty.translate G' Δ' (PTy i) = some (PTy' i)) ∧
+  --         ∃ (pats' : Vect n Core.Term),
+  --         (∀ i, Surface.Term.translate G' Δ' Γ' (pats i) = some (pats' i)) ∧
+  --         (∀ i, (pats' i).Determined) ∧
+  --         (∀ i, G'&Δ',Γ' ⊢ (pats' i) : (PTy' i)) := by
 
 
 
-    sorry
-  replace ih4 : ∃ (CTy' : Vect n Core.Ty),
-          (∀ (i : Fin n), Surface.Ty.translate G' Δ' (CTy i) = some (CTy' i)) ∧
-          ∃ (cs' : Vect n Core.Term),
-          (∀ i, Surface.Term.translate G' Δ' Γ' (cs i) = some (cs' i)) ∧
-          (∀ i, (cs' i).Determined) ∧
-          (∀ i, G'&Δ',Γ' ⊢ (cs' i) : (CTy' i)) := by
-    sorry
+  --   sorry
+  -- replace ih4 : ∃ (CTy' : Vect n Core.Ty),
+  --         (∀ (i : Fin n), Surface.Ty.translate G' Δ' (CTy i) = some (CTy' i)) ∧
+  --         ∃ (cs' : Vect n Core.Term),
+  --         (∀ i, Surface.Term.translate G' Δ' Γ' (cs i) = some (cs' i)) ∧
+  --         (∀ i, (cs' i).Determined) ∧
+  --         (∀ i, G'&Δ',Γ' ⊢ (cs' i) : (CTy' i)) := by
+  --   sorry
 
-  rcases ih3 with ⟨PTy', ih3a, ps', ih3b, ih3c, ih3d⟩
-  rcases ih4 with ⟨CTy', ih4a, cs', ih5b, ih5c, ih5d⟩
+  -- rcases ih3 with ⟨PTy', ih3a, ps', ih3b, ih3c, ih3d⟩
+  -- rcases ih4 with ⟨CTy', ih4a, cs', ih5b, ih5c, ih5d⟩
 
-  exists T'
-  apply And.intro
-  · assumption
-  · exists (match! s' ps' cs' c')
-    rw[Option.bind_eq_some_iff];
-    apply And.intro
-    · exists s';
-      apply And.intro
-      · assumption
-      · rw[Option.bind_eq_some_iff];
-        exists (λ i => ps' i)
-        rw[Option.bind_eq_some_iff]
-        apply And.intro
-        · unfold Vect.seq; simp;
-          split
-          · case _ ph _ =>
-             simp at *; cases ph;
-             case _ i ih3b' _ =>
-             replace ih3b := ih3b i
-             rw[ih3b] at ih3b'; simp at ih3b'
-          · simp; funext; case _ x =>
-            replace ih3b := ih3b x;
-            unfold Option.get;
-            split; case _ e1 e2 e3 e4 e5 e6 e7 =>
-            simp at *; rw[ih3b] at e6; cases e6; rfl
-        · exists (λ i => cs' i)
-          rw[Option.bind_eq_some_iff]
-          apply And.intro
-          · unfold Vect.seq; simp
-            split;
-            · case _ ph _ =>
-              simp at *; cases ph;
-              case _ i ih5b' _ =>
-              replace ih5b := ih5b i
-              rw[ih5b] at ih5b'; simp at ih5b'
-            · simp; funext; case _ x =>
-              replace ih5b := ih5b x;
-              unfold Option.get;
-              split; case _ e1 e2 e3 e4 e5 e6 e7 =>
-              simp at *; rw[ih5b] at e1; rw[ih5b] at e6; cases e6; rfl
-          · exists c'
-    · apply And.intro
-      · apply Core.Term.Determined.match; repeat assumption
-      · apply Core.Typing.mtch (CTy := CTy') (PTy := PTy') (pats := ps') (cs := cs')
-        assumption
-        apply Translation.ValidTyHeadVariable.sound wf h1 ih1 vhvR
-        assumption
-        intro i; apply Translation.ValidHeadVariable.sound wf h1 h2 h3 (ih3b i) (vhvps i)
-        apply ih3d
-        intro i; apply Translation.StableTypeMatch.sound (ih3a i) ih1 (stmPTys i)
-        apply ih5d
-        intro i;  apply Translation.PrefixTypeMatch.sound h2 (ih3a i) (ih4a i) ih2 (ptms i)
+  -- exists T'
+  -- apply And.intro
+  -- · assumption
+  -- · exists (match! s' ps' cs' c')
+  --   rw[Option.bind_eq_some_iff];
+  --   apply And.intro
+  --   · exists s';
+  --     apply And.intro
+  --     · assumption
+  --     · rw[Option.bind_eq_some_iff];
+  --       exists (λ i => ps' i)
+  --       rw[Option.bind_eq_some_iff]
+  --       apply And.intro
+  --       · unfold Vect.seq; simp;
+  --         split
+  --         · case _ ph _ =>
+  --            simp at *; cases ph;
+  --            case _ i ih3b' _ =>
+  --            replace ih3b := ih3b i
+  --            rw[ih3b] at ih3b'; simp at ih3b'
+  --         · simp; funext; case _ x =>
+  --           replace ih3b := ih3b x;
+  --           unfold Option.get;
+  --           split; case _ e1 e2 e3 e4 e5 e6 e7 =>
+  --           simp at *; rw[ih3b] at e6; cases e6; rfl
+  --       · exists (λ i => cs' i)
+  --         rw[Option.bind_eq_some_iff]
+  --         apply And.intro
+  --         · unfold Vect.seq; simp
+  --           split;
+  --           · case _ ph _ =>
+  --             simp at *; cases ph;
+  --             case _ i ih5b' _ =>
+  --             replace ih5b := ih5b i
+  --             rw[ih5b] at ih5b'; simp at ih5b'
+  --           · simp; funext; case _ x =>
+  --             replace ih5b := ih5b x;
+  --             unfold Option.get;
+  --             split; case _ e1 e2 e3 e4 e5 e6 e7 =>
+  --             simp at *; rw[ih5b] at e1; rw[ih5b] at e6; cases e6; rfl
+  --         · exists c'
+  --   · apply And.intro
+  --     · apply Core.Term.Determined.match; repeat assumption
+  --     · apply Core.Typing.mtch (CTy := CTy') (PTy := PTy') (pats := ps') (cs := cs')
+  --       assumption
+  --       apply Translation.ValidTyHeadVariable.sound wf h1 ih1 vhvR
+  --       assumption
+  --       intro i; apply Translation.ValidHeadVariable.sound wf h1 h2 h3 (ih3b i) (vhvps i)
+  --       apply ih3d
+  --       intro i; apply Translation.StableTypeMatch.sound (ih3a i) ih1 (stmPTys i)
+  --       apply ih5d
+  --       intro i;  apply Translation.PrefixTypeMatch.sound h2 (ih3a i) (ih4a i) ih2 (ptms i)
 
-theorem quantifier_magic {Δ : Surface.KindEnv} {Γ : Surface.TyEnv} {PTy : Fin n -> Surface.Ty} {pats : Vect n Surface.Term} :
-  Δ.translate = Δ' ->
-  Surface.TyEnv.translate G' Δ' Γ = some Γ' ->
-  (∀ (i : Fin n) {Δ' : Core.KindEnv} {Γ' : Core.TyEnv},
-    Δ.translate = Δ' →
-      Surface.TyEnv.translate G' Δ' Γ = some Γ' →
-        ∃ T',
-          Surface.Ty.translate G' Δ' (PTy i) = some T' ∧
-            ∃ t', Surface.Term.translate G' Δ' Γ' (pats i) = some t' ∧ t'.Determined ∧ G'&Δ',Γ' ⊢ t' : T') ->
-
- (∃ (PTy' : Fin n -> Core.Ty),
-          (∀ (i : Fin n),
-            Δ.translate = Δ' →
-            Surface.TyEnv.translate G' Δ' Γ = some Γ' →
-            Surface.Ty.translate G' Δ' (PTy i) = some (PTy' i))) ∧
- (∃ (pats' : Vect n Core.Term),
-       Δ.translate = Δ' →
-       Surface.TyEnv.translate G' Δ' Γ = some Γ' →
-   (∀ i, Surface.Term.translate G' Δ' Γ' (pats i) = some (pats' i))) ∧
- (∃ (pats' : Vect n Core.Term), (∀ i, (pats' i).Determined)) ∧
- (∃ (PTy' : Fin n -> Core.Ty), ∃ (pats' : Vect n Core.Term),
-      Δ.translate = Δ' →
-      Surface.TyEnv.translate G' Δ' Γ = some Γ' →
-   (∀ i, G'&Δ',Γ' ⊢ (pats' i) : (PTy' i))) := by
-intro h1 h2 h
--- have lem :
---   ∀ (i : Fin n) {Δ' : Core.KindEnv} {Γ' : Core.TyEnv},
---     Δ.translate = Δ' ->
---     Surface.TyEnv.translate G' Δ' Γ = some Γ' ->
---      (∃ T',
---       Δ.translate = Δ' →
+-- theorem quantifier_magic {Δ : Surface.KindEnv} {Γ : Surface.TyEnv} {PTy : Fin n -> Surface.Ty} {pats : Vect n Surface.Term} :
+--   Δ.translate = Δ' ->
+--   Surface.TyEnv.translate G' Δ' Γ = some Γ' ->
+--   (∀ (i : Fin n) {Δ' : Core.KindEnv} {Γ' : Core.TyEnv},
+--     Δ.translate = Δ' →
 --       Surface.TyEnv.translate G' Δ' Γ = some Γ' →
---       Surface.Ty.translate G' Δ' (PTy i) = some T') ∧
---      (∃ pats',
+--         ∃ T',
+--           Surface.Ty.translate G' Δ' (PTy i) = some T' ∧
+--             ∃ t', Surface.Term.translate G' Δ' Γ' (pats i) = some t' ∧ t'.Determined ∧ G'&Δ',Γ' ⊢ t' : T') ->
+
+--  (∃ (PTy' : Fin n -> Core.Ty),
+--           (∀ (i : Fin n),
+--             Δ.translate = Δ' →
+--             Surface.TyEnv.translate G' Δ' Γ = some Γ' →
+--             Surface.Ty.translate G' Δ' (PTy i) = some (PTy' i))) ∧
+--  (∃ (pats' : Vect n Core.Term),
 --        Δ.translate = Δ' →
 --        Surface.TyEnv.translate G' Δ' Γ = some Γ' →
---        Surface.Term.translate G' Δ' Γ' (pats i) = some pats') ∧
---      (∃ pats' : Vect n Core.Term, (pats' i).Determined) ∧
---      (∃ T', ∃ pats' : Vect n Core.Term,
---         Δ.translate = Δ' →
---         Surface.TyEnv.translate G' Δ' Γ = some Γ' →
---        G'&Δ',Γ' ⊢ (pats' i) : T') := by
---   intro i Δ' Γ' h1 h2
---   replace h := @h i Δ' Γ' h1 h2
---   rcases h with ⟨T', e1, pats', e2, e3, e4⟩
---   apply And.intro
---   exists T'; intros; assumption
---   apply And.intro
---   exists pats'; intros; assumption
---   apply And.intro
---   sorry
---   sorry
-apply And.intro
-· sorry
-· sorry
-
--- constructor
+--    (∀ i, Surface.Term.translate G' Δ' Γ' (pats i) = some (pats' i))) ∧
+--  (∃ (pats' : Vect n Core.Term), (∀ i, (pats' i).Determined)) ∧
+--  (∃ (PTy' : Fin n -> Core.Ty), ∃ (pats' : Vect n Core.Term),
+--       Δ.translate = Δ' →
+--       Surface.TyEnv.translate G' Δ' Γ = some Γ' →
+--    (∀ i, G'&Δ',Γ' ⊢ (pats' i) : (PTy' i))) := by
+-- intro h1 h2 h
+-- -- have lem :
+-- --   ∀ (i : Fin n) {Δ' : Core.KindEnv} {Γ' : Core.TyEnv},
+-- --     Δ.translate = Δ' ->
+-- --     Surface.TyEnv.translate G' Δ' Γ = some Γ' ->
+-- --      (∃ T',
+-- --       Δ.translate = Δ' →
+-- --       Surface.TyEnv.translate G' Δ' Γ = some Γ' →
+-- --       Surface.Ty.translate G' Δ' (PTy i) = some T') ∧
+-- --      (∃ pats',
+-- --        Δ.translate = Δ' →
+-- --        Surface.TyEnv.translate G' Δ' Γ = some Γ' →
+-- --        Surface.Term.translate G' Δ' Γ' (pats i) = some pats') ∧
+-- --      (∃ pats' : Vect n Core.Term, (pats' i).Determined) ∧
+-- --      (∃ T', ∃ pats' : Vect n Core.Term,
+-- --         Δ.translate = Δ' →
+-- --         Surface.TyEnv.translate G' Δ' Γ = some Γ' →
+-- --        G'&Δ',Γ' ⊢ (pats' i) : T') := by
+-- --   intro i Δ' Γ' h1 h2
+-- --   replace h := @h i Δ' Γ' h1 h2
+-- --   rcases h with ⟨T', e1, pats', e2, e3, e4⟩
+-- --   apply And.intro
+-- --   exists T'; intros; assumption
+-- --   apply And.intro
+-- --   exists pats'; intros; assumption
+-- --   apply And.intro
+-- --   sorry
+-- --   sorry
 -- apply And.intro
--- · intro i
---   replace h := @h i _ _ h1 h2
---   rcases h with ⟨T', h1, pat, h3, h4⟩
+-- · sorry
+-- · sorry
+
+-- -- constructor
+-- -- apply And.intro
+-- -- · intro i
+-- --   replace h := @h i _ _ h1 h2
+-- --   rcases h with ⟨T', h1, pat, h3, h4⟩
 
 
 
---   sorry
+-- --   sorry
 -- · sorry
 -- (intro i
 --  replace h := @h i _ _ h1 h2
