Core/Examples/Monad.lean
@@ -11,7 +11,7 @@ import Core.Typing
 namespace Core.Examples.Monad
 /- data Bool = True | False -/
 def BoolCtx : List Global := [
-  .data "Bool" ★ ([ ("True", gt#"Bool") , (("False"), gt#"Bool")]  : Vect 2 (String × Ty))
+  .data 2 "Bool" ★ ([ ("True", gt#"Bool") , (("False"), gt#"Bool")]  : Vect 2 (String × Ty))
   ]
 #guard Ty.infer_kind BoolCtx [] (gt#"Bool") == .some ★
 #guard Ty.infer_kind BoolCtx [] (gt#"Bool" -:> gt#"Bool" -:> gt#"Bool") == .some ★
@@ -24,7 +24,7 @@ not = λ x → case x of
                _ → False
 -/
 def notTerm : Term := λ[ .global "Bool" ]
-  match! #0
+  match! 2 #0
          [ g#"True", g#"False" ]
          ([ g# "False", g# "True" ] : Vect 2 Term)
          g#"False"
@@ -39,10 +39,10 @@ def notTerm : Term := λ[ .global "Bool" ]
                        False → True
  -/
 def eqBool : Term := λ[ .global "Bool" ] λ[ .global "Bool" ]
-  match!  #1
+  match! 2  #1
    [ g#"True", g#"False" ]
-   ([ match! #0 [ g#"True", g#"False" ] ([ g#"True", g#"False" ] : Vect 2 Term) g#"False",
-      match! #0 [ g#"True", g#"False" ] ([ g# "False", g# "False"] : Vect 2 Term) g#"False"
+   ([ match! 2 #0 [ g#"True", g#"False" ] ([ g#"True", g#"False" ] : Vect 2 Term) g#"False",
+      match! 2 #0 [ g#"True", g#"False" ] ([ g# "False", g# "False"] : Vect 2 Term) g#"False"
    ] : Vect 2 Term)
    g#"False"
 
@@ -54,7 +54,7 @@ def ListCtx : List Global := [
   -- data List a
   -- | Nil : ∀a. List a
   -- | Cons : ∀a. a → List a → List a
-  .data "List" (★ -:>  ★)
+  .data 2 "List" (★ -:>  ★)
   ([ ("Nil", ∀[★] (gt#"List" • t#0))
    , ("Cons", ∀[★] (t#0 -:> (gt#"List" • t#0) -:> (gt#"List" • t#0))) ] : Vect 2 (String × Ty)),
 
