Core/Examples/Nat.lean
@@ -7,8 +7,8 @@ import Core.Eval.BigStep
 import Core.Infer
 
 namespace Core.Examples.Bool
-def c1 := match! #0 [ g#"S" ]  ([ λ[gt#"Nat"] g#"False" ] : Vect 1 Term) g#"True"
-def c2 := λ[ gt#"Nat"] match! #1
+def c1 := match! 1 #0 [ g#"S" ]  ([ λ[gt#"Nat"] g#"False" ] : Vect 1 Term) g#"True"
+def c2 := λ[ gt#"Nat"] match! 1 #1
                        [ g#"S" ]
                        ([ λ[ gt#"Nat"] (g#"eq" • #1) • #0 ] : Vect 1 Term)
                        g#"False"
@@ -27,10 +27,10 @@ def NatCtxFix : List Global := [
 
   .inst "eq"
      (λ[ gt#"Nat"] λ[gt#"Nat"]
-        match! #1
+        match! 2 #1
         ([ g#"Z" , g#"S" ] : Vect 2 Term)
-        ([ match! #0 [ g#"S" ]  ([ λ[gt#"Nat"] g#"False" ] : Vect 1 Term) g#"True"
-         , λ[ gt#"Nat" ] match! #1
+        ([ match! 1 #0 [ g#"S" ]  ([ λ[gt#"Nat"] g#"False" ] : Vect 1 Term) g#"True"
+         , λ[ gt#"Nat" ] match! 1 #1
                        [ g#"S" ]
                        ([ λ[ gt#"Nat"] (g#"eq" • #1) • #0 ] : Vect 1 Term)
                        g#"False"
@@ -40,7 +40,7 @@ def NatCtxFix : List Global := [
 
   .openm "eq" (gt#"Nat" -:> gt#"Nat" -:> gt#"Bool"),
   -- Bool = True | False
-  .data "Bool" ★ ([ ("True", gt#"Bool"), ("False", gt#"Bool") ] : Vect 2 (String × Ty)),
+  .data 2 "Bool" ★ ([ ("True", gt#"Bool"), ("False", gt#"Bool") ] : Vect 2 (String × Ty)),
 
   -- two = add (S Z) (S Z)
   .defn "two" gt#"Nat" ((g#"add" • (g#"S" • g#"Z")) • (g#"S" • g#"Z")),
@@ -56,7 +56,7 @@ def NatCtxFix : List Global := [
         ((gt#"Nat" -:> gt#"Nat" -:> gt#"Nat") -:> gt#"Nat" -:> gt#"Nat" -:> gt#"Nat")
         (λ[ gt#"Nat" -:> gt#"Nat" -:> gt#"Nat"]
           λ[gt#"Nat"] λ[gt#"Nat"]
-            match! #1
+            match! 2 #1
               [ g#"Z", g#"S" ]
               ([ #0 ,
                  λ[ gt#"Nat" ] (g#"S" • ((#3 • #0) • #1)) ] : Vect 2 Term)
@@ -68,7 +68,7 @@ def NatCtxFix : List Global := [
   -- open fix : ∀ a, (a -> a) -> a
   .openm "fix" (∀[★] (t#0 -:> t#0) -:> t#0),
   -- data Nat = Z | Succ Nat
-  .data "Nat" ★ ([ ("Z", gt#"Nat"), ("S", gt#"Nat" -:> gt#"Nat") ] : Vect 2 (String × Ty))
+  .data 2 "Nat" ★ ([ ("Z", gt#"Nat"), ("S", gt#"Nat" -:> gt#"Nat") ] : Vect 2 (String × Ty))
 
 ]
 
