Core/Ty/Structure.lean
@@ -140,4 +140,50 @@ theorem Ty.Spine.apply_eta : ((gt#x).apply sp).spine = some (x, sp) := by
   have lem := @apply_compose x [] sp gt#x (by simp [Ty.spine])
   simp at lem; exact lem
 
+
+def Ty.is_all_some : Ty -> Option (Kind × Ty)
+| .all K B => return (K, B)
+| _ => none
+
+def Ty.is_all_some_sound {T : Ty} :
+  T.is_all_some = .some (K, T1) ->
+  T = ∀[K] T1 := by
+intro h
+cases T <;> simp [Ty.is_all_some] at *
+assumption
+
+
+def Ty.is_arrow_some : Ty -> Option (Ty × Ty)
+| .arrow A B => return (A, B)
+| _ => none
+
+def Ty.is_arrow_some_sound {T : Ty} :
+  T.is_arrow_some = .some (T1, T2) ->
+  T = T1 -:> T2 := by
+intro h
+cases T <;> simp [Ty.is_arrow_some] at *
+assumption
+
+def Ty.is_eq_some : Ty -> Option (Kind × Ty × Ty)
+| .eq K A B => return (K, A, B)
+| _ => none
+
+def Ty.is_eq_some_sound {T : Ty} :
+  T.is_eq_some = some (K, A, B) ->
+  T = (A ~[K]~ B) := by
+intro h;
+cases T <;> simp [Ty.is_eq_some] at *
+assumption
+
+def Ty.is_app_some : Ty -> Option (Ty × Ty)
+| .app A B => return (A, B)
+| _ => none
+
+def Ty.is_app_some_sound {T : Ty} :
+  T.is_app_some = some (A, B) ->
+  T = (A • B) := by
+intro h;
+cases T <;> simp [Ty.is_app_some] at *
+assumption
+
 end Core
